src/bigraphs.v
@@ -1,4 +1,4 @@
-From Coq Require Import Arith ZArith Psatz Bool
+(* From Coq Require Import Arith ZArith Psatz Bool
                         String List Program.Equality Program.Wf.
 Require Import Relations.
 Require Import Recdef.
@@ -435,4 +435,4 @@ Module UnGraphe.
 
 Definition leaf : Type := string * port. 
 
-End UnGraphe. *)
+End UnGraphe. *) *)
