src/propertiesbigraphs.v
@@ -1,0 +1,119 @@
+From Coq Require Import Arith ZArith Psatz Bool
+String List Program.Equality Program.Wf.
+Require Import Relations.
+Require Import Recdef.
+
+Require Import OrderedType.
+
+
+Set Warnings "-parsing".
+Unset Strict Implicit.
+Unset Printing Implicit Defensive.
+Set Warnings "parsing".
+
+Local Open Scope string_scope.
+Local Open Scope list_scope.
+Local Open Scope nat_scope.
+Local Open Scope bool_scope.
+Import ListNotations.
+
+
+Require Export Bool DecidableType OrderedType.
+Set Implicit Arguments.
+
+From MyProofs Require Import AlgebraBigraphs. 
+
+(*Definition Cmp (elt:Type)(cmp:elt->elt->bool) e1 e2 := cmp e1 e2 = true.
+
+
+Module Type WSfun (E : DecidableType).
+
+
+
+Section properties.
+Variable A : Type.
+
+Definition getIdNode {A : Type} (n : node A) : A :=
+  match n with Node (Id idn) => idn 
+  end.
+
+Definition eq_nodes {A : Type} (n1:node A) (n2:node A) : Prop :=
+    getIdNode n1 = getIdNode n2.
+
+Example v2b := Node (Id "v2").
+Example sameids : eq_nodes v0 v0.
+Proof. unfold eq_nodes. unfold getIdNode. simpl. reflexivity. Qed. 
+Example difIds : not (eq_nodes v0 v1).
+Proof. unfold eq_nodes. unfold getIdNode. simpl. discriminate. Qed. 
+
+Lemma eq_nodes_refl : forall A : Type, forall n : node A, eq_nodes n n.
+Proof. intros. unfold eq_nodes. unfold getIdNode. reflexivity. Qed.   
+
+Fixpoint getk (A:DecidableType) (n:node A) (c:control A) : option :=
+  match c with 
+    | [] => None
+    | (n', idk, k) :: q => if (eq_nodes n n') then Some k else getk n q
+  end. 
+
+End properties.
+
+Example k_v0: getk v0 mybig = Some 2.
+Proof. unfold getk. unfold getctrl. simpl. reflexivity. Qed.
+Example k_v1: getk v1 mybig = Some 2.
+Proof. unfold getk. unfold getctrl. simpl. reflexivity. Qed.
+Example k_v2: getk v2 mybig = Some 4.
+Proof. unfold getk. unfold getctrl. simpl. reflexivity. Qed.
+
+Fixpoint count_links_to_node {A: Type} (n:node A) (b:bigraph A) :=
+  0.
+
+*)
+  (** From the time with attachables*)
+(*Fixpoint count_ports_on_node_from_edges (atts:list attachables) (n:node) :=
+  match atts with 
+    | [] => 0
+    | a :: q => 
+      match a with
+        | AttachableNode an =>
+          if (equalsnodes an n)
+            then 1 + (count_ports_on_node_from_edges q n)
+            else (count_ports_on_node_from_edges q n)           
+        | _ => (count_ports_on_node_from_edges q n)
+      end
+  end.
+  
+  (*obligée d'utiliser le comme arg decreasing 
+    (*TODO*) foldleft <- existe déja *)
+Fixpoint count_ports_on_node_from_bigraph (b:bigraph) (n:node) (le: list edge) {struct le}:=
+  match le with
+  | [] => 0
+  | (Edge _ atts) :: es => 
+    (count_ports_on_node_from_edges atts n) +
+      (count_ports_on_node_from_bigraph (
+        Bigraph (getv b) es (getctrl b) (getprnt b) (getlnk b) (getk b) (getm b) (getx b) (gety b)) 
+        n
+        es
+      )
+  end.
+
+
+Fixpoint map (l:list node) (f: bigraph -> (k -> nat) -> node -> Prop) (b:bigraph) (ctrl: k -> nat) : Prop :=
+  match l with
+    | [] => True 
+    | a :: t => (f b ctrl a) /\ (map t f b ctrl)
+  end. 
+
+Fixpoint ctrl_for_one_node (b:bigraph) (ctrl: k -> nat) (n:node) : Prop :=
+  match n with
+    | Node id k => count_ports_on_node_from_bigraph b n (gete b) = ctrl k
+  end.
+
+Theorem control_respected : forall b:bigraph, match b with
+  | Bigraph v e ctrl prnt lnk k m x y => map v ctrl_for_one_node b ctrl 
+  end.
+Proof. intros. induction b.
+  - induction v.
+    + unfold map. reflexivity.
+    + unfold map. Admitted. 
+
+*)
