README.md
@@ -1,3 +1,12 @@
 # PFE
 
 Playground for my PFE
+
+
+To create CoqMakefile
+coq_makefile -f _CoqProject -o CoqMakefile
+
+
+To clean
+make -f CoqMakefile clean
+
